Adjust Case in thunk_cexp

compiler/backend/languages/semantics/thunk_exp_ofScript.sml
@@ -19,11 +19,22 @@ Definition lets_for_def:
         lets_for l cn v ws b
 End
 
+Overload True[local] = “Prim (Cons "True") []”;
+Overload False[local] = “Prim (Cons "False") []”;
+
+Definition Disj_def:
+  Disj v [] = False ∧
+  Disj v ((cn,l)::xs) = If (IsEq cn l T (Var v)) True (Disj v xs)
+End
+
 Definition rows_of_def:
-  rows_of v k [] = (k:thunkLang$exp) ∧
-  rows_of v k ((cn,vs,b)::rest) =
+  rows_of v [] k =
+    (case k of
+     | NONE => Prim (AtomOp Add) []
+     | SOME (alts,e) => If (Disj v alts) e Fail) ∧
+  rows_of v ((cn,vs,b)::rest) k =
     If (IsEq cn (LENGTH vs) T (Var v))
-      (lets_for (LENGTH vs) cn v (MAPi (λi v. (i,v)) vs) b) (rows_of v k rest)
+      (lets_for (LENGTH vs) cn v (MAPi (λi v. (i,v)) vs) b) (rows_of v rest k)
 End
 
 Definition op_of_def[simp]:
@@ -38,11 +49,11 @@ Definition exp_of_def[simp]:
   exp_of (App f xs)      = Apps (exp_of f) (MAP exp_of xs) ∧
   exp_of (Lam vs x)      = Lams (MAP explode vs) (exp_of x) ∧
   exp_of (Letrec rs x)   = Letrec (MAP (λ(n,x). (explode n,exp_of x)) rs) (exp_of x) ∧
-  exp_of (Case v rs opt) =
+  exp_of (Case v rs d) =
       rows_of
         (explode v)
-        (case opt of NONE => Fail | SOME e => exp_of e)
-        (MAP (λ(c,vs,x). (explode c,MAP explode vs,exp_of x)) rs) ∧
+        (MAP (λ(c,vs,x). (explode c,MAP explode vs,exp_of x)) rs)
+        (OPTION_MAP (λ(a,e). (MAP (explode ## I) a, exp_of e)) d) ∧
   exp_of (Force x)       = Force (exp_of x) ∧
   exp_of (Delay x)       = Delay (exp_of x) ∧
   exp_of (Box x)         = Box (exp_of x)
@@ -78,7 +89,7 @@ Definition cexp_wf_def:
     EVERY (λ(_,_,x). cexp_wf x) css ∧
     (eopt = NONE ⇒ css ≠ []) ∧
     ¬ MEM v (FLAT $ MAP (FST o SND) css) ∧
-    OPTION_ALL cexp_wf eopt ∧
+    OPTION_ALL (λ(_,e). cexp_wf e) eopt ∧
     (∀cn. MEM cn (MAP FST css) ⇒ explode cn ∉ monad_cns))
 Termination
   WF_REL_TAC ‘measure cexp_size’
